wip3

TM/Combinators/While.v
@@ -123,55 +123,34 @@ Section While.
   Qed.
 
 
-  (*
-  Lemma While_terminatesIn' t :
-
-    pM ↓(T) ->
-    (forall (x : tapes sig n) '(y, i),
-        T' x (y, i) -> exists (x':tapes _ _) (b:bool) i1 y1,
-           T x (y1,i1) /\ if b then exists i2 y2, T' x' (y2, i2) /\ i1+1+i2<=i else i1 <= i)->
-    WHILE ↓(T').
-  Proof.
-    intros Term_M Hyp. hnf.
-    intros t i. revert t. apply complete_induction with (x:=i); clear i; intros i IH t T't.
-    destruct (Hyp _ _ T't) as (t'& b& i1&Rx&Tx&H).
-    destruct b.
-    -destruct H as (i2&T't'&Leq).
-     apply IH in T't' as (oenc & Eq);[ |omega].
-     exists oenc.
-     apply Term_M in Tx as (oenc1 & Eq1).
-     apply (loop_ge (k1:=i1 + (1 + i2)));[omega| ].
-     specialize (HR _ _ _ Eq1). specialize (Func _ _ T't _ _ HR Rx). inv Func.
-     now apply (While_true_merge Eq1).
-    -apply Term_M in Tx as [oenc Eq].
-     exists oenc.
-     eapply While_false_merge. eapply loop_ge;[ |exact Eq]. omega.
-     specialize (HR _ _ _ Eq).
-     specialize (Func _ _ T't _ _ HR Rx). now inv Func.
-  Qed.
-*)
-
   Section WhileTerm.
 
-    Variable T : Rel (tapes sig n) (bool * tapes sig n * nat).
+    Variable T : Rel (tapes sig n) (mconfig sig (states (projT1 pM)) n * nat).
 
-    Inductive WhileTerm : Rel (tapes sig n) (unit * tapes sig n * nat) :=
-    | term_false i t1 t2      : T t1 (false, t2, i) -> WhileTerm t1 (tt, t2, i)
-    | term_true  i j t1 t2 t3 : T t1 (true, t2, i) -> WhileTerm t2 (tt, t3, j) -> WhileTerm t1 (tt, t3, i+1+j).
+    Inductive WhileTerm : (tapes sig n) -> (mconfig sig (states (projT1 pM)) n) -> nat -> Prop :=
+    | term_false (i : nat) (q : states (projT1 pM)) (t1 t2 : tapes sig n) :
+        T t1 (mk_mconfig q t2, i) ->
+        projT2 pM q = false ->
+        WhileTerm t1 (mk_mconfig q t2) i
+    | term_true (i j : nat) (q1 q2 : states (projT1 pM)) (t1 t2 t3 : tapes sig n) :
+        T t1 (mk_mconfig q1 t2, i) ->
+        projT2 pM q1 = true ->
+        WhileTerm t2 (mk_mconfig q2 t3) j ->
+        WhileTerm t1 (mk_mconfig q2 t3) (i + (1 + j)).
+
+    Definition WhileTerm' : Rel (tapes sig n) (mconfig sig (states (projT1 pM)) n * nat) :=
+      fun t '(c, k) => WhileTerm t c k.
+
+    Lemma While_Terminates :
+        projT1 pM ⇓ T -> While ⇓ WhileTerm'.
+    Proof.
+      intros Term. hnf. intros t1 t3 k H. unfold WhileTerm' in *.
+      induction H as [k q t1 t2 H1 H2 | i j q1 q2 t1 t2 t3 H1 H2 H3 H4].
+      - hnf in Term. specialize (Term t1 (mk_mconfig q t2) k H1). now apply While_false_merge.
+      - eapply While_true_merge; eauto.
+    Qed.
 
   End WhileTerm.
-  
-  
-  Lemma While_Terminates (T : Rel _ (bool * tapes sig n * nat)):
-    pM ⇓ T -> WHILE ⇓ WhileTerm T.
-  Proof.
-    intros Term. hnf. intros t1 t3 [] k.
-    induction 1.
-    - specialize (Term _ _ _ _ H) as (conf&Term&Term'&->). symmetry in Term'.
-      exists conf. pose proof While_false_merge Term Term' as L. repeat split; auto. cbn. auto.
-      + admit.
-  Qed.
-
 
 End While.
 (* Arguments While {n} {sig} M _. *)
